eve/Src/library/base/base2/dispenser/v_dispenser.e
@@ -1,0 +1,98 @@
+note
+	description: "Containers that can be extended with values and make only one element accessible at a time."
+	author: "Nadia Polikarpova"
+	model: sequence
+
+deferred class
+	V_DISPENSER [G]
+
+inherit
+	V_CONTAINER [G]
+
+feature -- Access
+
+	item: G
+			-- The accessible element.
+		require
+			not_empty: not is_empty
+			closed: closed
+			reads (ownership_domain)
+		deferred
+		ensure
+			definition: Result = sequence.first
+		end
+
+feature -- Iteration
+
+	new_cursor: V_ITERATOR [G]
+			-- New iterator pointing to the accessible element.
+			-- (Traversal in the order of accessibility.)
+		note
+			explicit: contracts
+			status: impure
+		deferred
+		ensure then
+			sequence_definition: Result.sequence ~ sequence
+		end
+
+feature -- Extension
+
+	extend (v: G)
+			-- Add `v' to the dispenser.
+		require
+			no_observers: observers.is_empty
+			modify_model ("sequence", Current)
+		deferred
+		ensure
+			bag_effect: bag ~ old (bag & v)
+		end
+
+feature -- Removal
+
+	remove
+			-- Remove the accessible element.
+		require
+			not_empty: not is_empty
+			no_observers: observers.is_empty
+			modify_model ("sequence", Current)
+		deferred
+		ensure
+			wrapped: is_wrapped
+			sequence_effect: sequence ~ old sequence.but_first
+		end
+
+	wipe_out
+			-- Remove all elements.
+		require
+			no_observers: observers.is_empty
+			modify_model ("sequence", Current)
+		deferred
+		ensure
+			wrapped: is_wrapped
+			sequence_effect: sequence.is_empty
+		end
+
+feature -- Specification
+
+	sequence: MML_SEQUENCE [G]
+			-- Sequence of elements in the order of access.
+		note
+			status: ghost
+			replaces: bag
+		attribute
+		end
+
+invariant
+	bag_definition: bag ~ sequence.to_bag
+	
+note
+	copyright: "Copyright (c) 1984-2014, Eiffel Software and others"
+	license: "Eiffel Forum License v2 (see http://www.eiffel.com/licensing/forum.txt)"
+	source: "[
+			Eiffel Software
+			5949 Hollister Ave., Goleta, CA 93117 USA
+			Telephone 805-685-1006, Fax 805-685-6869
+			Website http://www.eiffel.com
+			Customer support http://support.eiffel.com
+		]"
+end
