eve/Src/library/base/base2/dispenser/v_linked_stack.e
@@ -1,0 +1,142 @@
+note
+	description: "Linked implementation of stacks."
+	author: "Nadia Polikarpova"
+	model: sequence
+
+frozen class
+	V_LINKED_STACK [G]
+
+inherit
+	V_STACK [G]
+		redefine
+			default_create,
+			forget_iterator
+		end
+
+feature {NONE} -- Initialization
+
+	default_create
+			-- Create an empty stack.
+		note
+			status: creator
+		do
+			create list
+			set_owns ([list])
+		ensure then
+			sequence_effect: sequence.is_empty
+		end
+
+feature -- Initialization
+
+	copy_ (other: like Current)
+			-- Initialize by copying all the items of `other'.
+		require
+			no_observers: observers.is_empty
+			modify_model ("sequence", Current)
+			modify_model ("closed", other)
+		do
+			if other /= Current then
+				other.unwrap
+				list.copy_ (other.list)
+				other.wrap
+			end
+		ensure then
+			sequence_effect: sequence ~ other.sequence
+		end
+
+feature -- Access
+
+	item: G
+			-- The top element.
+		do
+			check inv end
+			check list.transitive_owns <= transitive_owns end
+			Result := list.first
+		end
+
+feature -- Measurement
+
+	count: INTEGER
+			-- Number of elements.
+		do
+			check inv end
+			Result := list.count
+			check list.inv_only ("count_definition") end
+		end
+
+feature -- Iteration
+
+	new_cursor: V_LINKED_STACK_ITERATOR [G]
+			-- New iterator pointing to a position in the container, from which it can traverse all elements by going `forth'.
+		note
+			status: impure
+			explicit: contracts
+		local
+			list_cursor: V_LINKED_LIST_ITERATOR [G]
+		do
+			unwrap
+			list_cursor := list.new_cursor
+			create Result.make (Current, list_cursor)
+			wrap
+		end
+
+feature -- Extension
+
+	extend (v: G)
+			-- Push `v' on the stack.
+		do
+			list.extend_front (v)
+			check sequence.prepended (v) = sequence.old_.extended_at (1, v) end
+		end
+
+feature -- Removal
+
+	remove
+			-- Pop the top element.
+		do
+			list.remove_front
+		end
+
+	wipe_out
+			-- Pop all elements.
+		do
+			list.wipe_out
+		end
+
+feature {V_CONTAINER, V_ITERATOR} -- Implementation
+
+	list: V_LINKED_LIST [G]
+			-- Underlying list.
+			-- Should not be reassigned after creation.
+
+feature -- Specification
+
+	forget_iterator (it: like new_cursor)
+			-- Remove `it' from `observers'.
+		note
+			status: ghost
+			explicit: contracts
+		do
+			it.unwrap
+			set_observers (observers / it)
+			list.forget_iterator (it.iterator)
+		end
+
+invariant
+	list_exists: list /= Void
+	owns_definition: owns = [list]
+	sequence_definition: sequence ~ list.sequence
+	observers_correspond: observers.count = list.observers.count
+
+note
+	explicit: observers, owns
+	copyright: "Copyright (c) 1984-2014, Eiffel Software and others"
+	license: "Eiffel Forum License v2 (see http://www.eiffel.com/licensing/forum.txt)"
+	source: "[
+			Eiffel Software
+			5949 Hollister Ave., Goleta, CA 93117 USA
+			Telephone 805-685-1006, Fax 805-685-6869
+			Website http://www.eiffel.com
+			Customer support http://support.eiffel.com
+		]"
+end
