eve/Src/library/base/base2/dispenser/v_stack.e
@@ -1,0 +1,80 @@
+note
+	description: "Dispensers where the latest added element is accessible."
+	author: "Nadia Polikarpova"
+	model: sequence
+
+deferred class
+	V_STACK [G]
+
+inherit
+	V_DISPENSER [G]
+		redefine
+			extend
+		end
+
+feature -- Comparison
+
+	is_equal_ (other: like Current): BOOLEAN
+			-- Is stack made of the same values in the same order as `other'?
+			-- (Use reference comparison.)
+		note
+			status: impure
+		require
+			modify_model ("observers", [Current, other])
+		local
+			i, j: V_ITERATOR [G]
+		do
+			check inv and other.inv end
+			if other = Current then
+				Result := True
+			elseif count = other.count then
+				from
+					Result := True
+					i := new_cursor
+					j := other.new_cursor
+				invariant
+					1 <= i.index_ and i.index_ <= sequence.count + 1
+					i.index_ = j.index_
+					Result implies across create {MML_INTERVAL}.from_range (1, i.index_ - 1) as k all sequence [k.item] = other.sequence [k.item] end
+					not Result implies sequence [i.index_ - 1] /= other.sequence [i.index_ - 1]
+					i.is_wrapped and j.is_wrapped
+					modify_model ("index_", [i, j])
+				until
+					i.after or not Result
+				loop
+					check across create {MML_INTERVAL}.from_range (1, i.index_ - 1) as k all sequence [k.item] = other.sequence [k.item] end end
+					Result := i.item = j.item
+					i.forth
+					j.forth
+				variant
+					sequence.count - i.index_
+				end
+				check Result implies across create {MML_INTERVAL}.from_range (1, i.index_ - 1) as k all sequence [k.item] = other.sequence [k.item] end end
+				forget_iterator (i)
+				other.forget_iterator (j)
+			end
+		ensure then
+			definition: Result = (sequence ~ other.sequence)
+			observers_restored: observers ~ old observers
+		end
+
+feature -- Extension
+
+	extend (v: G)
+			-- Push `v' on the stack.
+		deferred
+		ensure then
+			sequence_effect: sequence ~ old sequence.prepended (v)
+		end
+		
+note
+	copyright: "Copyright (c) 1984-2014, Eiffel Software and others"
+	license: "Eiffel Forum License v2 (see http://www.eiffel.com/licensing/forum.txt)"
+	source: "[
+			Eiffel Software
+			5949 Hollister Ave., Goleta, CA 93117 USA
+			Telephone 805-685-1006, Fax 805-685-6869
+			Website http://www.eiffel.com
+			Customer support http://support.eiffel.com
+		]"
+end
