eve/Src/library/base/base2/iterator/dispenser/v_linked_stack_iterator.e
@@ -1,0 +1,166 @@
+note
+	description: "Iterators over linked stacks."
+	author: "Nadia Polikarpova"
+	model: target, sequence, index_
+
+class
+	V_LINKED_STACK_ITERATOR [G]
+
+inherit
+	V_ITERATOR [G]
+		redefine
+			target
+		end
+
+create {V_CONTAINER}
+	make
+
+feature {NONE} -- Initialization
+
+	make (t: V_LINKED_STACK [G]; it: V_LINKED_LIST_ITERATOR [G])
+			-- Create a proxy for `it' with target `t'.
+		note
+			status: creator
+			explicit: contracts
+		require
+			t_wrapped: t.is_open
+			it_wrapped: it.is_wrapped
+			it_target_owned: t.owns [it.target]
+			same_elements: t.bag ~ it.target.bag
+			modify_field ("owner", it)
+			modify_field ("observers", t)
+			modify (Current)
+		do
+			target := t
+			t.set_observers (t.observers & Current)
+			iterator := it
+			check it.inv end
+		ensure
+			is_wrapped
+			target_effect: target = t
+			sequence_effect: sequence ~ it.sequence
+			index_effect: index_ = it.index_
+			t_observers_effect: t.observers = old t.observers & Current
+		end
+
+feature -- Access
+
+	target: V_LINKED_STACK [G]
+
+	item: G
+			-- Item at current position.
+		do
+			check inv end
+			check iterator.inv end
+			check iterator.target.transitive_owns <= target.transitive_owns end
+			Result := iterator.item
+		end
+
+feature -- Measurement		
+
+	index: INTEGER
+			-- Current position.
+		do
+			check inv end
+			check iterator.inv end
+			check iterator.target.transitive_owns <= target.transitive_owns end
+			Result := iterator.index
+		end
+
+feature -- Status report
+
+	before: BOOLEAN
+			-- Is current position before any position in `target'?
+		do
+			check inv end
+			check iterator.inv end
+			Result := iterator.before
+		end
+
+	after: BOOLEAN
+			-- Is current position after any position in `target'?
+		do
+			check inv end
+			check iterator.inv end
+			Result := iterator.after
+		end
+
+	is_first: BOOLEAN
+			-- Is cursor at the first position?
+		do
+			check inv end
+			check iterator.inv end
+			check iterator.target.transitive_owns <= target.transitive_owns end
+			Result := iterator.is_first
+		end
+
+	is_last: BOOLEAN
+			-- Is cursor at the last position?
+		do
+			check inv end
+			check iterator.inv end
+			check iterator.target.transitive_owns <= target.transitive_owns end
+			Result := iterator.is_last
+		end
+
+feature -- Cursor movement
+
+	start
+			-- Go to the first position.
+		do
+			iterator.start
+		end
+
+	finish
+			-- Go to the last position.
+		do
+			iterator.finish
+		end
+
+	forth
+			-- Move one position forward.
+		do
+			iterator.forth
+		end
+
+	back
+			-- Go one position backwards.
+		do
+			iterator.back
+		end
+
+	go_before
+			-- Go before any position of `target'.
+		do
+			iterator.go_before
+		end
+
+	go_after
+			-- Go after any position of `target'.
+		do
+			iterator.go_after
+		end
+
+feature {V_CONTAINER, V_ITERATOR} -- Implementation
+
+	iterator: V_LINKED_LIST_ITERATOR [G]
+			-- Iterator over the storage.
+
+invariant
+	iterator_exists: iterator /= Void
+	owns_structure: owns = [ iterator ]
+	targets_connected: target.owns [iterator.target]
+	same_sequence: sequence ~ iterator.sequence
+	same_index: index_ = iterator.index_
+
+note
+	copyright: "Copyright (c) 1984-2014, Eiffel Software and others"
+	license: "Eiffel Forum License v2 (see http://www.eiffel.com/licensing/forum.txt)"
+	source: "[
+			Eiffel Software
+			5949 Hollister Ave., Goleta, CA 93117 USA
+			Telephone 805-685-1006, Fax 805-685-6869
+			Website http://www.eiffel.com
+			Customer support http://support.eiffel.com
+		]"
+end
